\section{Appendix}
\textit{This section includes the MATLAB function codes and additional support materials.}

\subsection{Appendix A - Angle-Axis to Rotation Matrix}
\begin{verbatim}
function R = AngleAxisToRot(h, theta)
    % Normalize the axis vector
    h = h / norm(h);
    
    % Construct the skew-symmetric matrix
    K = [0, -h(3), h(2);
         h(3), 0, -h(1);
         -h(2), h(1), 0];
         
    % Identity matrix
    I = eye(3);
    
    % Calculate the rotation matrix using the Rodrigues formula
    R = I + sin(theta) * K + (1 - cos(theta)) * (K * K);
end
\end{verbatim}

\subsection{Appendix B - Yaw-Pitch-Roll to Rotation Matrix}
\begin{verbatim}
function R = YPRToRot(psi, theta, phi)
    % Calculate the individual rotation matrices
    R_z = [cos(psi), -sin(psi), 0;
           sin(psi), cos(psi), 0;
           0, 0, 1];
       
    R_y = [cos(theta), 0, sin(theta);
           0, 1, 0;
           -sin(theta), 0, cos(theta)];
       
    R_x = [1, 0, 0;
           0, cos(phi), -sin(phi);
           0, sin(phi), cos(phi)];
    
    % Combine the rotation matrices
    R = R_z * R_y * R_x;
end
\end{verbatim}

\subsection{Appendix C - Rotation Matrix to Euler Angles}
\begin{verbatim}
function [psi, theta, phi] = RotToYPR(R)
    % Check for the valid rotation matrix
    assert(abs(det(R) - 1) < 1e-6, 'Invalid rotation matrix');
    
    % Calculate yaw, pitch, and roll angles
    theta = asin(-R(3,1));
    
    if cos(theta) > 1e-6
        psi = atan2(R(2,1), R(1,1));
        phi = atan2(R(3,2), R(3,3));
    else
        psi = atan2(-R(1,2), R(1,1));
        phi = 0;
    end
end
\end{verbatim}

\subsection{Appendix D - Rotation Matrix to Angle-Axis}
\begin{verbatim}
function [h, theta] = RotToAngleAxis(R)
    % Check for a valid rotation matrix
    assert(abs(det(R) - 1) < 1e-6, 'Invalid rotation matrix');
    
    theta = acos((trace(R) - 1) / 2);
    if theta == 0
        h = [1; 0; 0]; % Default axis
    else
        h = [(R(3,2) - R(2,3)) / (2 * sin(theta));
             (R(1,3) - R(3,1)) / (2 * sin(theta));
             (R(2,1) - R(1,2)) / (2 * sin(theta))];
    end
end
\end{verbatim}
